Zcash/Circuits.lean
@@ -84,7 +84,6 @@ import Zcash.Circuits.Action.RealBases
 import Zcash.Circuits.Action.Spec
 import Clean.Halo2.TopLevel
 import Zcash.Circuits.Action.TopLevel
-import Zcash.Circuits.Action.SelectorCoherence
 import Zcash.Circuits.Integration
 
 /-!
